Split HeapExtend stuff in own theory

Denotational-Common.thy
@@ -130,106 +130,19 @@ proof
   show "?lhs \<Longrightarrow> ?rhs" using imp[of "\<pi> \<bullet> h" "\<pi> \<bullet> f" "-\<pi>"] by simp
 qed
 
-definition heapExtendMeet :: "Env \<Rightarrow> heap \<Rightarrow> (exp \<Rightarrow> Env \<Rightarrow> Value)  \<Rightarrow> (var, Value) fmap"
-  where
-  "heapExtendMeet \<rho> h eval =
-    (if (\<forall>e \<in> snd ` set h. cont (eval e)) \<and> compatible_fmap \<rho> (heapToEnv h (\<lambda> e. eval e \<rho>) )
-    then fmap_meet \<rho> (fixR (fmap_bottom (fst ` set h)) (\<lambda> \<rho>' . heapToEnv h (\<lambda> e. eval e (fmap_meet \<rho> \<rho>'))))
-    else fempty)"
 
-lemma heapExtendMeet_eqvt[eqvt]:
-  "\<pi> \<bullet> heapExtendMeet \<rho> h eval = heapExtendMeet (\<pi> \<bullet> \<rho>) (\<pi> \<bullet> h) (\<pi> \<bullet> eval)"
-proof (cases "(\<forall> e \<in> snd ` set h. cont (eval e)) \<and> compatible_fmap \<rho> (heapToEnv h (\<lambda> e. eval e \<rho>))")
-  case True
-  moreover hence "(\<forall> e \<in> snd ` set (\<pi> \<bullet> h). cont ((\<pi> \<bullet> eval) e)) \<and> compatible_fmap (\<pi> \<bullet> \<rho>) (heapToEnv (\<pi> \<bullet> h) (\<lambda> e. (\<pi> \<bullet> eval) e (\<pi> \<bullet> \<rho>))) " sorry
-  ultimately show ?thesis
-   unfolding heapExtendMeet_def
-   apply -
-   apply (subst if_P, assumption)+
-   apply (subst fmap_meet_eqvt)
-   apply (subst fixR_eqvt)
-   apply (auto simp add: fmap_bottom_eqvt)[1]
-   apply perm_simp
-   apply rule
-   done
-next
-case False thus ?thesis
-   unfolding heapExtendMeet_def
-   apply (subst if_not_P, assumption)
-   apply (subst if_not_P)
-   apply  (rule notI)
-   apply  (erule notE)
-   apply  rule
-   apply  (metis perm_still_cont4)
-   apply  (erule conjE)
-   apply  (drule compatible_fmap_eqvt[of _ _ "- \<pi>"])
-   apply  (simp add: permute_fun_def heapToEnv_eqvt)
-   apply (rule fempty_eqvt)
-   done
-qed
-
-lemma heapExtendMeet_cong[fundef_cong]:
-  "\<lbrakk> env1 = env2 ; heap1 = heap2 ;  (\<And> e. e \<in> snd ` set heap2 \<Longrightarrow> eval1 e = eval2 e) \<rbrakk>
-      \<Longrightarrow> heapExtendMeet env1 heap1 eval1 = heapExtendMeet env2 heap2 eval2"
-  unfolding heapExtendMeet_def
-  by (auto cong:heapToEnv_cong)
-
-definition heapExtend :: "Env \<Rightarrow> heap \<Rightarrow> (exp \<Rightarrow> Env \<Rightarrow> Value)  \<Rightarrow> (var, Value) fmap"
-  where
-  "heapExtend \<rho> h eval =
-    (if (\<forall>e \<in> snd ` set h. cont (eval e))
-    then fmap_update \<rho> (fix1 (fmap_bottom (fst ` set h)) (\<Lambda> \<rho>' . heapToEnv h (\<lambda> e. eval e (fmap_update \<rho> \<rho>'))))
-    else fempty)"
-
-
-lemma heapExtend_eqvt[eqvt]:
-  "\<pi> \<bullet> heapExtend \<rho> h eval = heapExtend (\<pi> \<bullet> \<rho>) (\<pi> \<bullet> h) (\<pi> \<bullet> eval)"
-proof (cases "\<forall> e \<in> snd ` set h. cont (eval e)")
-  case True
-  moreover hence "\<forall> e \<in> snd ` set (\<pi> \<bullet> h). cont ((\<pi> \<bullet> eval) e)" by (simp only: perm_still_cont4 simp_thms(35))
-  ultimately show ?thesis
-   unfolding heapExtend_def
-   apply -
-   apply (subst if_P, assumption)+
-   apply (subst fmap_update_eqvt)
-   apply (subst fix1_eqvt)
-   apply (subst Lam_eqvt)
-     apply (rule cont2cont)
-     apply (rule cont_compose) back
-     apply auto[1]
-     apply auto[1]
-    apply (auto simp add: fmap_bottom_eqvt)[1]
-    apply perm_simp
-    apply rule
-    done
-next
-case False thus ?thesis
-   unfolding heapExtend_def
-   apply (simp_all only: if_not_P perm_still_cont4)
-   apply auto
-  done 
-qed
-
-lemma heapExtend_cong[fundef_cong]:
-  "\<lbrakk> env1 = env2 ; heap1 = heap2 ;  (\<And> e. e \<in> snd ` set heap2 \<Longrightarrow> eval1 e = eval2 e) \<rbrakk>
-      \<Longrightarrow> heapExtend env1 heap1 eval1 = heapExtend env2 heap2 eval2"
-  unfolding heapExtend_def
-  by (auto cong:heapToEnv_cong)
-
-lemma heapExtend_cont[simp,cont2cont]: "cont (\<lambda>\<rho>. heapExtend \<rho> h eval)"
-  unfolding heapExtend_def
-  apply (cases "\<forall> e \<in> snd ` set h.  cont (eval e)")
-  apply (simp_all only: if_P if_not_P perm_still_cont4 simp_thms(35) if_False)
-  apply (intro cont2cont)
-  apply (rule cont_compose[where c = "eval e", standard, where eval = eval]) 
-  apply auto[1]
+lemma lookupHeapToEnvE:
+  assumes "v \<in> fst ` set h"
+  obtains e where "(v, e) \<in> set h" and "\<And> f. the (lookup (heapToEnv h f) v) = f e"
+  using assms
+  apply rule
+  apply (induct h)
   apply simp
-  apply (subst beta_cfun)
-  apply (intro cont2cont)
-  apply (rule cont_compose[where c = "eval e", standard, where eval = eval]) 
-  apply auto[1]
-  apply simp
-  apply simp
-  apply simp
+  apply auto
+  defer
+  apply (case_tac "a = aa")
+  apply auto
   done
+
+
 end
