Denotational-Compatible.thy
@@ -1,0 +1,169 @@
+theory "Denotational-Compatible"
+  imports "Denotational-Common" "HOLCF-Set-Nominal" "FMap-Nominal-HOLCF"
+begin
+
+
+lemmas fdom_perm_rev[eqvt]
+
+lemma below_eqvt [eqvt]:
+    "\<pi> \<bullet> (x \<sqsubseteq> y) = (\<pi> \<bullet> x \<sqsubseteq> \<pi> \<bullet> (y::'a::cont_pt))" by (auto simp add: permute_pure)
+
+nominal_primrec
+  compatible_with_exp :: "exp \<Rightarrow> Env \<Rightarrow> Env set" 
+  and
+  compatible_with_heap :: "heap \<Rightarrow> Env \<Rightarrow> Env set"
+where
+  "compatible_with_exp (Var v) d = {\<rho>' . d \<sqsubseteq> \<rho>'}" |
+  "atom x \<sharp> d \<Longrightarrow> compatible_with_exp (Lam [x]. e) d = compatible_with_exp e d" |
+  "compatible_with_exp (App e x) d = compatible_with_exp e d" |
+  "compatible_with_exp (Let as body) d = compatible_with_exp body d \<inter> compatible_with_heap (asToHeap as) d" |
+
+  "compatible_with_heap [] d = {\<rho>' . d \<sqsubseteq> \<rho>'}" |
+  "compatible_with_heap (x # xs) d = compatible_with_heap xs d" (* TODO. Was hier? *)
+proof-
+case goal1 thus ?case
+  unfolding compatible_with_exp_compatible_with_heap_graph_def eqvt_def
+  apply rule
+  apply perm_simp
+  apply rule
+  done
+next
+case (goal3 P x)
+  show ?case
+  proof (cases x)
+  case (Inl y)
+    show ?thesis
+    proof(cases y)
+    case (Pair e d)
+      show ?thesis
+      using Inl Pair goal3
+        apply (rule_tac y=e in exp_assn.exhaust(1))
+        apply blast+
+        apply (rule_tac y=e and c = d in exp_assn.strong_exhaust(1), auto simp add: fresh_star_singleton, metis)[1]
+        done
+    qed
+  next
+  case (Inr y)
+    show ?thesis
+    proof(cases y)
+    case (Pair h d)
+      show ?thesis
+      apply (cases h)
+      using Inr Pair goal3
+      apply blast+
+      done
+   qed
+qed
+next
+apply_end auto
+next
+  fix X show X X X X X X sorry
+qed
+
+termination(eqvt) by lexicographic_order
+
+lemma ESem_cont_induct_lemma:
+  "subpcpo (compatible_with_exp e d) &&& bottom_of (compatible_with_exp e d) = d"
+  and
+  "subpcpo (compatible_with_heap (asToHeap as) d) &&& bottom_of (compatible_with_heap (asToHeap as) d) = d"
+proof(nominal_induct e and avoiding: d rule:exp_assn.strong_induct)
+print_cases
+  case (Var v d)
+  show "subpcpo (compatible_with_exp (Var v) d)"
+    by (simp, rule subpcpo_cone_above)
+  show "bottom_of (compatible_with_exp (Var v) d) = d" by simp
+next
+  case (App e x d)
+    case 1 thus ?case using App by auto
+    case 2 thus ?case using App by auto
+next
+  case (Lam x e d)
+    case 1 thus ?case using Lam by auto
+    case 2 thus ?case using Lam by auto
+next
+  case (Let as body d)
+    case 1 thus ?case
+      using Let by (auto intro: subpcpo_inter)
+    case 2 thus ?case using Let apply simp by (metis bottom_of_inter)
+next
+  case ANil
+    case 1 thus ?case apply simp
+qed
+
+lemma heap_compat_subset:
+   "e \<in> snd ` set h \<Longrightarrow> compatible_with_heap h d \<subseteq> compatible_with_exp e d" sorry
+
+lemma compat_fdom [simp]: "\<rho> \<in> compatible_with_heap h d \<Longrightarrow> fdom \<rho> = fdom d" sorry
+
+lemma compatible_with_heap_is_subpcpo:
+  "subpcpo (compatible_with_heap h d)" sorry
+
+lemma bottom_is_compatible:
+  "fmap_bottom d \<in> compatible_with_exp e (fmap_bottom d)"
+  "fmap_bottom d \<in> compatible_with_heap h (fmap_bottom d)" sorry
+
+definition compatible_with_heap_and_env
+  where "compatible_with_heap_and_env h eval \<rho> = {\<rho>' . \<rho>' \<in> compatible_with_heap h (fmap_bottom (fdom \<rho> \<union> (fst ` set h))) \<and> compatible_fmap \<rho> (heapToEnv h (\<lambda> e. eval e \<rho>')) }"
+
+lemma compatible_disjoint_is_subpcpo:
+  fixes \<rho> :: "Env"
+  and eval :: "exp \<Rightarrow> Env \<Rightarrow> Value"
+  assumes bot: "compatible_fmap \<rho> (heapToEnv h (\<lambda> e. eval e (fmap_bottom (fdom \<rho> \<union> fst ` set h))))"
+  and e_sub: "\<And> e. e \<in> snd ` set h \<Longrightarrow> subpcpo (compatible_with_exp e (fmap_bottom (fdom \<rho> \<union> fst ` set h)))"
+  and e_cont: "\<And> e. e \<in> snd ` set h \<Longrightarrow> cont_on (compatible_with_exp e (fmap_bottom (fdom \<rho> \<union> fst ` set h))) (eval e)"
+  shows "subpcpo (compatible_with_heap_and_env h eval \<rho>)" (is "subpcpo ?S")
+proof(rule subpcpoI)
+  let ?dom = "fmap_bottom (fdom \<rho> \<union> fst ` set h)"
+  fix Y :: "nat \<Rightarrow> Env"
+  assume "chain Y"
+  assume "\<And> i. Y i \<in> ?S"
+  show "(\<Squnion> i. Y i) \<in> ?S"
+  proof(subst compatible_with_heap_and_env_def, rule,rule)
+    show "(\<Squnion> i. Y i) \<in> compatible_with_heap h ?dom"
+      using `\<And> i. Y i \<in> ?S`
+      by (auto simp add: compatible_with_heap_and_env_def subpcpo.pcpo[OF compatible_with_heap_is_subpcpo] `chain Y`)
+    next
+    show "compatible_fmap \<rho> (heapToEnv h (\<lambda>e. eval e (\<Squnion> i. Y i))) "
+    proof(rule compatible_fmapI)
+      fix v
+      assume dom1: "v \<in> fdom \<rho>"
+      assume dom2: "v \<in> fdom (heapToEnv h (\<lambda>e. eval e (\<Squnion> i. Y i)))"
+      hence "v \<in> fst ` set h" by auto
+      then obtain e where "(v, e) \<in> set h" and e: "\<And>\<rho>' . the (lookup (heapToEnv h (\<lambda>e. eval e \<rho>')) v) = eval e \<rho>'"
+          by (metis lookupHeapToEnvE)
+      hence "e \<in> snd ` set h" by (metis imageI snd_conv)
+      then interpret subpcpo "compatible_with_exp e ?dom" by (rule e_sub)
+
+      from `chain Y` and `\<And> i. Y i \<in> ?S`
+      have "chain_on (compatible_with_exp e ?dom) Y"
+        by (auto intro: chain_onI chainE[OF `chain Y`] subsetD[OF heap_compat_subset[OF `e \<in> _`]] simp add: compatible_with_heap_and_env_def)
+
+      have "compatible (the (lookup \<rho> v)) (eval e (\<Squnion> i. Y i))"
+      thm adm_onD admD
+      proof (rule adm_onD)
+        fix i
+        have "Y i \<in> ?S" by fact
+        hence "compatible_fmap \<rho> (heapToEnv h (\<lambda>e. eval e (Y i)))" by (auto simp add: compatible_fmap_def' compatible_with_heap_and_env_def)
+        hence "compatible (the (lookup \<rho> v)) (the (lookup (heapToEnv h (\<lambda>e. eval e (Y i))) v))"
+          unfolding compatible_fmap_def' using dom1 dom2 by auto
+        thus "compatible (the (lookup \<rho> v)) (eval e (Y i))" using e by metis
+        next
+        show "adm_on (compatible_with_exp e ?dom) (\<lambda>a. compatible (the (lookup \<rho> v)) (eval e a))"
+          by (rule adm_on_subst[OF subpcpo_axioms subpcpo_UNIV e_cont[OF `e \<in> _`] subset_UNIV subpcpo.adm_is_adm_on[OF subpcpo_UNIV compatible_adm]])          
+      qed fact
+
+      thus "compatible (the (lookup \<rho> v)) (the (lookup (heapToEnv h (\<lambda>e. eval e (\<Squnion> i. Y i))) v))"
+        by (auto simp add: e)
+    qed
+  qed
+next
+  show "fmap_bottom (fdom \<rho> \<union> (fst ` set h)) \<in> ?S" (is "?bot \<in> _")
+    by (auto intro: bottom_is_compatible bot simp add: compatible_with_heap_and_env_def)
+  fix y
+  assume "y \<in> ?S"
+  thus "?bot \<sqsubseteq> y"
+    by (auto intro: fmap_bottom_below simp add: compatible_with_heap_and_env_def)
+qed
+
+
+end
