Denotational-HeapExtend.thy
@@ -1,0 +1,151 @@
+theory "Denotational-HeapExtend"
+  imports "Denotational-Common" "Denotational-Compatible"
+begin
+
+definition heapExtendMeet :: "Env \<Rightarrow> heap \<Rightarrow> (exp \<Rightarrow> Env \<Rightarrow> Value)  \<Rightarrow> (var, Value) fmap"
+  where
+  "heapExtendMeet \<rho> h eval =
+    (if (\<forall>e \<in> snd ` set h. cont (eval e)) \<and> compatible_fmap \<rho> (heapToEnv h (\<lambda> e. eval e \<rho>) )
+    then fmap_meet \<rho> (fixR (fmap_bottom (fst ` set h)) (\<lambda> \<rho>' . heapToEnv h (\<lambda> e. eval e (fmap_meet \<rho> \<rho>'))))
+    else fempty)"
+
+lemma heapExtendMeet_def2:
+  "heapExtendMeet \<rho> h eval =
+    (if (\<forall>e \<in> snd ` set h. cont (eval e)) \<and> compatible_fmap \<rho> (heapToEnv h (\<lambda> e. eval e \<rho>) )
+    then (fixR (fmap_bottom (fdom \<rho> \<union> fst ` set h)) (\<lambda> \<rho>' . fmap_meet \<rho> (heapToEnv h (\<lambda> e. eval e \<rho>'))))
+    else fempty)" (is "_ = (if _ then fixR ?x2 ?F2 else _)")
+proof (cases "(\<forall> e \<in> snd ` set h. cont (eval e)) \<and> compatible_fmap \<rho> (heapToEnv h (\<lambda> e. eval e \<rho>))")
+case True
+  let "fixR ?x1 ?F1" = "fixR (fmap_bottom (fst ` set h)) (\<lambda> \<rho>'. heapToEnv h (\<lambda> e. eval e (fmap_meet \<rho> \<rho>')))"
+  show ?thesis
+  proof(induct rule: below_antisym[case_names lt gt])
+  case lt
+    have "fmap_meet \<rho> (fixR ?x1 ?F1) \<sqsubseteq> fixR (?F2 ?x2) ?F2"
+      apply (rule parallel_fixR_ind)
+      sorry also
+    have "... = fixR ?x2 ?F2" sorry
+    finally show ?case unfolding heapExtendMeet_def using True by auto
+  next
+  case gt
+    have "fixR ?x2 ?F2  \<sqsubseteq> fmap_meet \<rho> (fixR ?x1 ?F1)"
+      sorry
+    thus ?case unfolding heapExtendMeet_def using True by auto
+  qed
+next
+case False
+  thus ?thesis unfolding heapExtendMeet_def apply (subst if_not_P, assumption)+ ..
+qed
+
+
+definition heapExtendMeed_cond
+  where "heapExtendMeed_cond h eval \<rho> = 
+    (compatible_fmap \<rho> (heapToEnv h (\<lambda> e. eval e (fmap_bottom (fdom \<rho> \<union> fst ` set h)))) \<and> 
+    (\<forall> e \<in> snd ` set h. subpcpo (compatible_with_exp e (fdom \<rho> \<union> fst ` set h))) \<and>
+    (\<forall> e \<in> snd ` set h. cont_on (compatible_with_exp e (fdom \<rho> \<union> fst ` set h)) (eval e)))"
+
+
+lemma heapExtendMeet_def3:
+  "heapExtendMeet \<rho> h eval =
+    (if heapExtendMeed_cond h eval \<rho>
+    then fix_on (compatible_with_heap_and_env h eval \<rho>) (\<lambda> \<rho>'. fmap_meet \<rho> (heapToEnv h (\<lambda> e. eval e \<rho>')))
+    else fempty)"
+sorry
+
+
+lemma heapExtendMeet_eqvt[eqvt]:
+  "\<pi> \<bullet> heapExtendMeet \<rho> h eval = heapExtendMeet (\<pi> \<bullet> \<rho>) (\<pi> \<bullet> h) (\<pi> \<bullet> eval)"
+proof (cases "(\<forall> e \<in> snd ` set h. cont (eval e)) \<and> compatible_fmap \<rho> (heapToEnv h (\<lambda> e. eval e \<rho>))")
+  case True
+  moreover hence "(\<forall> e \<in> snd ` set (\<pi> \<bullet> h). cont ((\<pi> \<bullet> eval) e)) \<and> compatible_fmap (\<pi> \<bullet> \<rho>) (heapToEnv (\<pi> \<bullet> h) (\<lambda> e. (\<pi> \<bullet> eval) e (\<pi> \<bullet> \<rho>))) " sorry
+  ultimately show ?thesis
+   unfolding heapExtendMeet_def
+   apply -
+   apply (subst if_P, assumption)+
+   apply (subst fmap_meet_eqvt)
+   apply (subst fixR_eqvt)
+   apply (auto simp add: fmap_bottom_eqvt)[1]
+   apply perm_simp
+   apply rule
+   done
+next
+case False thus ?thesis
+   unfolding heapExtendMeet_def
+   apply (subst if_not_P, assumption)
+   apply (subst if_not_P)
+   apply  (rule notI)
+   apply  (erule notE)
+   apply  rule
+   apply  (metis perm_still_cont4)
+   apply  (erule conjE)
+   apply  (drule compatible_fmap_eqvt[of _ _ "- \<pi>"])
+   apply  (simp add: permute_fun_def heapToEnv_eqvt)
+   apply (rule fempty_eqvt)
+   done
+qed
+
+lemma heapExtendMeet_cong[fundef_cong]:
+  "\<lbrakk> env1 = env2 ; heap1 = heap2 ;  (\<And> e. e \<in> snd ` set heap2 \<Longrightarrow> eval1 e = eval2 e) \<rbrakk>
+      \<Longrightarrow> heapExtendMeet env1 heap1 eval1 = heapExtendMeet env2 heap2 eval2"
+  unfolding heapExtendMeet_def
+  by (auto cong:heapToEnv_cong)
+
+definition heapExtend :: "Env \<Rightarrow> heap \<Rightarrow> (exp \<Rightarrow> Env \<Rightarrow> Value)  \<Rightarrow> (var, Value) fmap"
+  where
+  "heapExtend \<rho> h eval =
+    (if (\<forall>e \<in> snd ` set h. cont (eval e))
+    then fmap_update \<rho> (fix1 (fmap_bottom (fst ` set h)) (\<Lambda> \<rho>' . heapToEnv h (\<lambda> e. eval e (fmap_update \<rho> \<rho>'))))
+    else fempty)"
+
+
+lemma heapExtend_eqvt[eqvt]:
+  "\<pi> \<bullet> heapExtend \<rho> h eval = heapExtend (\<pi> \<bullet> \<rho>) (\<pi> \<bullet> h) (\<pi> \<bullet> eval)"
+proof (cases "\<forall> e \<in> snd ` set h. cont (eval e)")
+  case True
+  moreover hence "\<forall> e \<in> snd ` set (\<pi> \<bullet> h). cont ((\<pi> \<bullet> eval) e)" by (simp only: perm_still_cont4 simp_thms(35))
+  ultimately show ?thesis
+   unfolding heapExtend_def
+   apply -
+   apply (subst if_P, assumption)+
+   apply (subst fmap_update_eqvt)
+   apply (subst fix1_eqvt)
+   apply (subst Lam_eqvt)
+     apply (rule cont2cont)
+     apply (rule cont_compose) back
+     apply auto[1]
+     apply auto[1]
+    apply (auto simp add: fmap_bottom_eqvt)[1]
+    apply perm_simp
+    apply rule
+    done
+next
+case False thus ?thesis
+   unfolding heapExtend_def
+   apply (simp_all only: if_not_P perm_still_cont4)
+   apply auto
+  done 
+qed
+
+lemma heapExtend_cong[fundef_cong]:
+  "\<lbrakk> env1 = env2 ; heap1 = heap2 ;  (\<And> e. e \<in> snd ` set heap2 \<Longrightarrow> eval1 e = eval2 e) \<rbrakk>
+      \<Longrightarrow> heapExtend env1 heap1 eval1 = heapExtend env2 heap2 eval2"
+  unfolding heapExtend_def
+  by (auto cong:heapToEnv_cong)
+
+
+lemma heapExtend_cont[simp,cont2cont]: "cont (\<lambda>\<rho>. heapExtend \<rho> h eval)"
+  unfolding heapExtend_def
+  apply (cases "\<forall> e \<in> snd ` set h.  cont (eval e)")
+  apply (simp_all only: if_P if_not_P perm_still_cont4 simp_thms(35) if_False)
+  apply (intro cont2cont)
+  apply (rule cont_compose[where c = "eval e", standard, where eval = eval]) 
+  apply auto[1]
+  apply simp
+  apply (subst beta_cfun)
+  apply (intro cont2cont)
+  apply (rule cont_compose[where c = "eval e", standard, where eval = eval]) 
+  apply auto[1]
+  apply simp
+  apply simp
+  apply simp
+  done
+end
